F*/F* tutorial/Ex7.fst
@@ -65,3 +65,44 @@ val step : exp -> Tot (option exp)
         | Some e1' -> Some (EIf e1' e2 e3)
         | None     -> None)
   | _ -> None
+
+let _ = assert (step (EApp (EAbs 0 TBool (EVar 0)) ETrue) = Some ETrue)
+let _ = assert (step (EApp ETrue ETrue) = None)
+
+type test = i : int{i > 0}
+
+type env = int -> Tot (option ty)
+
+val empty : env
+let empty = fun _ -> None
+
+val extend : env -> int -> ty -> Tot env
+let extend g x t = fun x' -> if x = x' then Some t else g x'
+
+val typing : env -> exp -> Tot (option ty)
+let rec typing g e =
+  match e with
+  | EVar x -> g x
+  | EAbs x t e1 ->
+      (match typing (extend g x t) e1 with
+      | Some t' -> Some (TArrow t t')
+      | None    -> None)
+  | EApp e1 e2 ->
+      (match typing g e1, typing g e2 with
+      | Some (TArrow t11 t12), Some t2 -> if t11 = t2 then Some t12 else None
+      | _                    , _       -> None)
+  | ETrue  -> Some TBool
+  | EFalse -> Some TBool
+  | EIf e1 e2 e3 ->
+      (match typing g e1, typing g e2, typing g e3 with
+      | Some TBool, Some t2, Some t3 -> if t2 = t3 then Some t2 else None
+      | _         , _      , _       -> None)
+
+val progress : e:exp → Lemma (requires (Some? (typing empty e)))
+                             (ensures (is_value e \/ (Some? (step e))))
+let rec progress = function
+  | EApp e1 e2   -> progress e1; progress e2
+  | EIf e1 e2 e3 -> progress e1; progress e2; progress e3
+  | _            -> ()
+
+
